properties.v
@@ -2,6 +2,7 @@
 Require Import Coq.Lists.List.
 Open Scope list_scope.
 Import ListNotations.
+Require Import Coq.Program.Equality.
 Require Import Resources.utility.
 Require Import Resources.name.
 Require Import Resources.type.
@@ -10,417 +11,89 @@ Require Import Resources.memory.
 Require Import Resources.instr.
 Require Import Resources.small_step.
 
-Definition pre_tag_consistent (s : state) : Prop :=
-  ∀ (r1 r2 : Resource),
-    state_contains_r s r1 →
-    state_contains_r s r2 →
-    tag_of r1 = tag_of r2 →
-    r1 = r2.
+Definition stack_tag_u (s : LocalStack) : Prop := ∀ t (p1 p2 : lstack_contains_t s t), p1 = p2.
 
-Theorem step_preserve_tag_consistent :
-∀ (s0 s1 : state),
-  pre_tag_consistent s0 →
-  step s0 s1 →
-  pre_tag_consistent s1.
-Proof.
-intros s0 s1 Hc Hs.
-destruct Hs as [s0 s1 i].
-unfold pre_tag_consistent.
-inversion H.
-+ admit.
-+ intros.
-  unfold pre_tag_consistent in Hc. 
-    (* r1, r2 on stack or in mem? *)
-    inversion H6; inversion H7.
-    {
-      (* both in mem  *)
-      apply Hc.
-      {
-        apply state_mem_contains.
-        rewrite H0.
-        assumption.
-      }
-      {
-        apply state_mem_contains.
-        rewrite H0.
-        assumption.
-      }
-      {
-        assumption.
-      }
-    }
-    {
-      (* r1 on mem, r2 on stack *)
-      subst.
-      apply Hc.
-      {
-        apply state_mem_contains.
-        rewrite H0.
-        assumption.
-      }
-      {
-        apply state_stack_contains.
-        rewrite <- H4 in H12.
-        apply stack_contains_cons_u in H12.
-        assumption.
-      }
-      {
-        assumption.
-      }
-    }
-    {
-      (* r1 on mem, r2 on stack *)
-      subst.
-      apply Hc.
-      {
-        apply state_stack_contains.
-        rewrite <- H4 in H9.
-        apply stack_contains_cons_u in H9.
-        assumption.
-      }
-      {
-        apply state_mem_contains.
-        rewrite H0.
-        assumption.
-      }
-      {
-        assumption.
-      }
-    }
-    {
-      subst.
-      apply Hc.
-      {
-        apply state_stack_contains.
-        rewrite <- H4 in H9.
-        apply stack_contains_cons_u in H9.
-        assumption.
-      }
-      {
-        apply state_stack_contains.
-        rewrite <- H4 in H12.
-        apply stack_contains_cons_u in H12.
-        assumption.
-      }
-      {
-        assumption.
-      }
-    }
-  ++ intros.
-    unfold tag_consistent in Hc. destruct Hc as [_ Hc].
-    (* destruct s0.
-    destruct s1.
-    simpl in *.
-    subst.
-    destruct p1. *)
-    destruct p1; destruct p2.
-    {
-      subst.
-      destruct s.
-      simpl in *.
-      subst.
-      assert (m = m0). {
-      remember (state_mem_contains s0 r m0) as m0'.
-      remember (state_mem_contains s0 r m) as m'.
-      pose proof (Hc r m0' m').
-      rewrite Heqm0' in H0.
-      rewrite Heqm' in H0.
-      apply foo in H0.
-      symmetry.
-      assump
+Definition mem_tag_u (m : Memory) : Prop := ∀ t (p1 p2 : mem_contains_t m t), p1 = p2.
 
+Definition notc (s : Set) : Prop := s → False.
 
-Definition tag_consistent (s : state) : Prop :=
-  (∀ (r1 r2 : Resource),
-    state_contains_r s r1 →
-    state_contains_r s r2 →
-    tag_of r1 = tag_of r2 →
-    r1 = r2) ∧
-  (∀ (r : Resource) (p1 p2 : state_contains_r s r), p1 = p2).
+Definition stack_mem_disjoint_tag m s : Prop :=
+  (∀ t, mem_contains_t m t → notc (lstack_contains_t s t)) ∧
+  (∀ t, lstack_contains_t s t → notc (mem_contains_t m t)).
 
-Lemma stack_contains_cons_u : ∀ (u : UnrestrictedValue) s r,
-  lstack_contains_r (val u :: s) r →
-  lstack_contains_r s r.
+Definition tag_uniq s : Set :=
+  mem_tag_u s.(mem) ∧
+  stack_tag_u s.(stack) ∧
+  stack_mem_disjoint_tag s.(mem) s.(stack).
+
+Lemma stack_contains_t_cons_u : ∀ (u : UnrestrictedValue) s t,
+  lstack_contains_t (val u :: s) t →
+  lstack_contains_t s t.
 Proof.
   intros.
   inversion H.
   assumption.
-Qed.
+Defined.
 
-Lemma foo s :
-(∀ (r : Resource) (p1 p2 : state_contains_r s r), p1 = p2) →
-(∀ r (p1 p2 : mem_contains_r s.(mem) r), p1 = p2).
-Proof.
-  intros.
-  remember (s.(mem)) as mem.
-  remember (s.(stack)) as stack.
-  remember (state_mem_contains mem r p1 stack) as x.
-  remember (state_mem_contains mem r p2 stack) as y.
-  assert (s = {| mem := mem; stack := stack |}). {
-    rewrite Heqmem. rewrite Heqstack.
-    destruct s.
-    simpl.
-    reflexivity.
-  }
-  rewrite <- H0 in x.
-  specialize H with r x y.
-  rewrite Heqx in H.
-  rewrite Heqy in H.
-  inversion H.
-  inversion H1.
-  inversion (existT (λ s : state, {r : Resource & mem_contains_r (mem s) r}) s
-  (existT (λ r : Resource, mem_contains_r (mem s) r) r p1) ).
-  simpl in H1.
-  intuition.
-  auto.
-  destruct x.
-
-(* Inductive state_contains_r' : state → Resource → Set :=
-  | state_mem_contains : ∀ m s r, mem_contains_r m r → state_contains_r' {|
-    mem := m;
-    stack := s;
-  |} r
-  | state_stack_contains : ∀ s r, lstack_contains_r s.(stack) r → state_contains_r' s r
-. *)
-
-Lemma foo : ∀ s r x y, state_mem_contains s r x = state_mem_contains s r y → x = y.
-Proof.
-  intros.
-  destruct (state_mem_contains s r x) eqn:E1.
-  inversion H.
-  + 
-  destruct (state_mem_contains s r x) eqn:E1; destruct (state_mem_contains s r y) eqn:E2.
-  +  
-  - destruct (state_mem_contains s r y) eqn:E2.
-    + assert (x0 = x) as Hx. { apply (mem_contains_r_proof_uniq s.(mem) r); auto. }
-      assert (x0 = y) as Hy. { apply (mem_contains_r_proof_uniq s.(mem) r); auto. }
-      rewrite Hx, Hy. reflexivity.
-    + discriminate H.
-  - destruct (state_mem_contains s r y) eqn:E2.
-    + discriminate H.
-    + reflexivity.
-Qed.
-
-Lemma foo : ∀ s r x y, state_mem_contains s r x = state_mem_contains s r y → x = y.
-Proof.
-  intros.
-  inversion H.
-Admitted.
-
-Theorem step_preserve_tag_consistent :
+Proposition step_preserve_stack_tag_u :
 ∀ (s0 s1 : state),
-  tag_consistent s0 →
-  step s0 s1 →
-  tag_consistent s1.
+tag_uniq s0 →
+step s0 s1 →
+stack_tag_u s1.(stack).
 Proof.
-  intros s0 s1 Hc Hs.
+  intros s0 s1 [Hm [Hu Hd]] Hs.
   destruct Hs as [s0 s1 i].
-  unfold tag_consistent.
+  unfold stack_tag_u in Hu.
+  unfold stack_tag_u.
   inversion H.
-  + admit.
-  + split.
-    ++ intros.
-      unfold tag_consistent in Hc. destruct Hc as [Hc _].
-      (* r1, r2 on stack or in mem? *)
-      inversion H6; inversion H7.
+  + destruct v.
+    ++
+      destruct v.
       {
-        (* both in mem  *)
-        apply Hc.
-        {
-          apply state_mem_contains.
-          rewrite H0.
-          assumption.
-        }
-        {
-          apply state_mem_contains.
-          rewrite H0.
-          assumption.
-        }
-        {
-          assumption.
-        }
-      }
-      {
-        (* r1 on mem, r2 on stack *)
-        subst.
-        apply Hc.
-        {
-          apply state_mem_contains.
-          rewrite H0.
-          assumption.
-        }
-        {
-          apply state_stack_contains.
-          rewrite <- H4 in H12.
-          apply stack_contains_cons_u in H12.
-          assumption.
-        }
-        {
-          assumption.
-        }
+        intros.
+        dependent destruction p1; dependent destruction p2.
+        + enough (r1 = r2).
+          rewrite H6.
+          reflexivity.
+          unfold mem_tag_u in Hm.
+          destruct s0.
+          simpl in *.
+          destruct mem.
+          unfold maps_var_to in H5.
+          simpl in *.
+          subst.
+          remember local as L. remember global as G.
+          remember (local_mem_ct L G t (local_mem_contains_tc L x r H5 t r1)) as p1.
+          remember (local_mem_ct L G t (local_mem_contains_tc L x r H5 t r2)) as p2.
+          specialize Hm with t p1 p2.
+          subst.
+          dependent destruction Heqp2.
+          reflexivity.
+        + admit.
+        + admit.
+        + specialize Hu with t p1 p2.
+          rewrite Hu.
+          reflexivity.
       }
       {
-        (* r1 on mem, r2 on stack *)
-        subst.
-        apply Hc.
-        {
-          apply state_stack_contains.
-          rewrite <- H4 in H9.
-          apply stack_contains_cons_u in H9.
-          assumption.
-        }
-        {
-          apply state_mem_contains.
-          rewrite H0.
-          assumption.
-        }
-        {
-          assumption.
-        }
-      }
-      {
-        subst.
-        apply Hc.
-        {
-          apply state_stack_contains.
-          rewrite <- H4 in H9.
-          apply stack_contains_cons_u in H9.
-          assumption.
-        }
-        {
-          apply state_stack_contains.
-          rewrite <- H4 in H12.
-          apply stack_contains_cons_u in H12.
-          assumption.
-        }
-        {
-          assumption.
-        }
-      }
-    ++ intros.
-      unfold tag_consistent in Hc. destruct Hc as [_ Hc].
-      (* destruct s0.
-      destruct s1.
-      simpl in *.
-      subst.
-      destruct p1. *)
-      destruct p1; destruct p2.
-      {
-       subst.
-       destruct s.
-       simpl in *.
-       subst.
-       assert (m = m0). {
-        remember (state_mem_contains s0 r m0) as m0'.
-        remember (state_mem_contains s0 r m) as m'.
-        pose proof (Hc r m0' m').
-        rewrite Heqm0' in H0.
-        rewrite Heqm' in H0.
-        apply foo in H0.
-        symmetry.
-        assumption.
-       }
-       rewrite H0.
-       reflexivity.
-      }
-      {
-
-      }
-      }
-      apply Hc.
-
-Theorem step_preserve_tag_consistent' :
-∀ (s0 s1 : state),
-  tag_consistent' s0 →
-  step s0 s1 →
-  tag_consistent' s1.
-Proof.
-  intros s0 s1 Hc Hs.
-  destruct s0. destruct s1.
-  destruct Hs.
-  inversion H.
-  + admit.
-  (* cploc *)
-  + unfold tag_consistent'. intros.
-    destruct l1; destruct l2.
-      ++ assert (state_maps_to s0 (inl r) c1). {
-        apply state_maps_to_mem_compat1 in H6.
-        apply state_maps_to_mem_compat0.
-        rewrite H0.
-        assumption.
-      } assert (state_maps_to s0 (inl r0) c2). {
-        apply state_maps_to_mem_compat1 in H7.
-        apply state_maps_to_mem_compat0.
-        rewrite H0.
-        assumption.
-      }
-      unfold tag_consistent' in Hc.
-      apply Hc with (l1:=inl r) (l2:=inl r0) (c1:=c1) (c2:=c2); assumption.
-      ++ unfold tag_consistent' in Hc.
-        apply state_maps_to_mem_compat1 in H6.
-        rewrite <- H0 in H6.
-        apply state_maps_to_mem_compat0 in H6.
-        apply state_maps_to_stack_compat1 in H7.
-        rewrite <- H4 in H7.
-        destruct s.
-        destruct stack_root0.
-        {
-          apply stack_maps_to_car1 in H7.
-          destruct H7. destruct H7. destruct H7.
-          inversion H7.
-          contradiction.
-        }
-        {
-          apply stack_maps_to_cdr in H7.
-          destruct H7. destruct H7. destruct H7.
-          inversion H7.
-          rewrite <- H12 in H9.
-          apply state_maps_to_stack_compat0 in H9.
-          specialize Hc with (l1 := inl r) (l2 := inr {| stack_root := stack_root0; stack_path := stack_path0 |}) (c1:=c1) (c2:=c2).
-          apply Hc in H6; auto.
-          inversion H6.
-        }
-      ++ unfold tag_consistent' in Hc.
-        apply state_maps_to_mem_compat1 in H7.
-        rewrite <- H0 in H7.
-        apply state_maps_to_mem_compat0 in H7.
-        apply state_maps_to_stack_compat1 in H6.
-        rewrite <- H4 in H6.
-        destruct s.
-        destruct stack_root0.
-        {
-          apply stack_maps_to_car1 in H6.
-          destruct H6. destruct H6. destruct H6.
-          inversion H6.
-          contradiction.
-        }
-        {
-          apply stack_maps_to_cdr in H6.
-          destruct H6. destruct H6. destruct H6.
-          inversion H6.
-          rewrite <- H12 in H9.
-          apply state_maps_to_stack_compat0 in H9.
-          specialize Hc with (l2 := inl r) (l1 := inr {| stack_root := stack_root0; stack_path := stack_path0 |}) (c1:=c1) (c2:=c2).
-          apply Hc in H7; auto.
-          inversion H7.
-        }
-      ++ unfold tag_consistent' in Hc.
-        apply state_maps_to_stack_compat1 in H6.
-        apply state_maps_to_stack_compat1 in H7.
-        rewrite <- H4 in H6, H7.
-        destruct s.
-        apply stack_maps_to_u_cons in H6.
-        destruct H6. destruct H6.
-        apply state_maps_to_stack_compat0 in H9.
-        destruct s2.
-        apply stack_maps_to_u_cons in H7.
-        destruct H7. destruct H7.
-        apply state_maps_to_stack_compat0 in H10.
-        specialize Hc with (l1 := (inr {| stack_root := x0; stack_path := stack_path0 |})) (l2 := (inr {| stack_root := x1; stack_path := stack_path1 |}))
-        (c1 := c1) (c2 := c2).
-        apply Hc in H9; auto.
-        rewrite <- H6.
-        rewrite <- H7.
-        inversion H9.
+        intros.
+        dependent destruction p1.
+        dependent destruction p2.
+        specialize Hu with t p1 p2.
+        rewrite Hu.
         reflexivity.
+      }
+    (* x -> ref *)
+    ++ intros.
+      dependent destruction p1.
+      dependent destruction p2.
+      specialize Hu with t p1 p2.
+      rewrite Hu.
+      reflexivity.
+  + intros.
+    dependent destruction p1.
+    dependent destruction p2.
+    specialize Hu with t p1 p2.
+    rewrite Hu.
+    reflexivity.
 Admitted.
